\begin{solution}
\begin{enumerate}
\item {[12 points]} If $v\in C^2_D[0,1]$, then
\[
-\int_0^1p''(x)v(x)\,dx=\int_0^1f(x)v(x)\,dx.
\]
Integration by parts then yields that
\[
-[p'(x)v(x)]_0^1+\int_0^1p'(x)v'(x)\,dx=\int_0^1f(x)v(x)\,dx
\]
from which we can conclude that
\[
p'(0)v(0)+\int_0^1p'(x)v'(x)\,dx=\int_0^1f(x)v(x)\,dx
\]
since $v(1)=0$. Hence,
\[
-\alpha v(0)+\int_0^1p'(x)v'(x)\,dx=\int_0^1f(x)v(x)\,dx
\]
since $-p'(0)=\alpha$. Therefore,
\[
\int_0^1p'(x)v'(x)\,dx=q(f,\alpha,v)\mbox{ for all }v\in C^2_D[0,1]
\]
where
\[
q(f,\alpha,v)=\int_0^1f(x)v(x)\,dx+\alpha v(0).
\]
\\
\item {[13 points]} If $v\in C^2[0,1]$, then
\[
\int_0^1\left(-4u''(x)+9u(x)\right)v(x)\,dx=\int_0^1f(x)v(x)\,dx
\]
since
\[
-4u''(x)+9u(x)=f(x),\quad 0<x<1.
\]
Integration by parts then yields that
\begin{eqnarray*}
&&\int_0^1\left(-4u''(x)+9u(x)\right)v(x)\,dx
\\
&=&-4\int_0^1u''(x)v(x)\,dx+9\int_0^1u(x)v(x)\,dx
\\
&=&-4\left[u'(x)v(x)\right]_0^1+4\int_0^1u'(x)v'(x)\,dx+9\int_0^1u(x)v(x)\,dx
\\
&=&-4u'(1)v(1)-\left(-4u'(0)v(0)\right)+\int_0^1\left(4u'(x)v'(x)+9u(x)v(x)\right)\,dx
\end{eqnarray*}
from which we can conclude that
\[
-\beta v(1)-\alpha v(0)+\int_0^1\left(4u'(x)v'(x)+9u(x)v(x)\right)\,dx=\int_0^1f(x)v(x)\,dx
\]
since $-4u'(0)=\alpha$ and $4u'(1)=\beta$. Therefore,
\[
\int_0^1\left(4u'(x)v'(x)+9u(x)v(x)\right)\,dx=g(f,\alpha,\beta,v)\mbox{ for all }v\in C^2[0,1]
\]
where
\[
g(f,\alpha,\rho,v)=\int_0^1f(x)v(x)\,dx+\alpha v(0)+\beta v(1).
\]
\end{enumerate}
\end{solution}