\begin{solution}
\begin{enumerate}
\item {[6 points]} If $f\in C[-1,1]$ then
\[
(P_e f)(x) = {1 \over 2}\left(f(x)+f(-x)\right)
\]
and so
\begin{eqnarray*}
(P_e(P_e f))(x) &=& {1 \over 2}\left((P_ef)(x)+(P_ef)(-x)\right)
\\
&=& \displaystyle{{1 \over 2}\left({1\over 2}\left(f(x)+f(-x)\right)+{1 \over 2}\left(f(-x)+f(-(-x))\right)\right)}
\\
&=& = \displaystyle{{1 \over 2}\left({1\over 2}f(x)+{1\over 2}f(-x)+{1 \over 2}f(-x)+{1\over 2}f(x)\right)}
\\
&=& {1 \over 2}\left(f(x)+f(-x)\right)
\\
&=& (P_e f)(x).
\end{eqnarray*}
Thus we conclude that $P_e(P_e f) = P_e f$ for all $f\in C[-1,1]$ which means that $P_e$ is a projection. In the same way, if $f\in C[-1,1]$ then
\[
(P_o f)(x) = {1 \over 2}\left(f(x)-f(-x)\right)
\]
and so
\begin{eqnarray*}
(P_o(P_o f))(x) &=& {1 \over 2}\left((P_of)(x)-(P_of)(-x)\right)
\\
&=& \displaystyle{{1 \over 2}\left({1\over 2}\left(f(x)-f(-x)\right)-{1 \over 2}\left(f(-x)-f(-(-x))\right)\right)}
\\
&=& \displaystyle{{1 \over 2}\left({1\over 2}f(x)-{1\over 2}f(-x)-{1 \over 2}f(-x)+{1\over 2}f(x)\right)}
\\
&=& {1 \over 2}\left(f(x)-f(-x)\right)
\\
&=& (P_o f)(x).
\end{eqnarray*}
Thus we conclude that $P_o(P_o f) = P_o f$ for all $f\in C[-1,1]$, which means that $P_o$ is a also projection.
\\
\item {[6 points]} If $f\in C[-1,1]$ then
\begin{eqnarray*}
\ip{P_e f, P_o f} &=& \int_{-1}^1 (P_e f)(x) (P_o f)(x)\, d x
\\
&=& \int_{-1}^1 {1\over 4}\left(f(x)+f(-x)\right)\left(f(x)-f(-x)\right)\, d x
\\
&=& {1\over 4} \int_{-1}^1 \left(\left(f(x)\right)^2 - f(x) f(-x) + f(x) f(-x) - \left(f(-x)\right)^2\right)  \, dx
\\
&=& {1\over 4} \int_{-1}^1 \left(\left(f(x)\right)^2 - \left(f(-x)\right)^2\right)  \, dx
\\
&=& {1\over 4} \left(\int_{-1}^1 \left(f(x)\right)^2 \, dx - \int_{-1}^1 \left(f(-x)\right)^2  \, dx\right)
\\
&=& {1\over 4} \left(\int_{-1}^1 \left(f(x)\right)^2 \, dx + \int_{-(-1)}^{-1} \left(f(y)\right)^2  \, dy\right)
\\
&=& {1\over 4} \left(\int_{-1}^1 \left(f(x)\right)^2 \, dx + \int_1^{-1} \left(f(y)\right)^2  \, dy\right)
\\
&=& {1\over 4} \left(\int_{-1}^1 \left(f(x)\right)^2 \, dx - \int_{-1}^1 \left(f(y)\right)^2  \, dy\right)
\\
&=& 0
\end{eqnarray*}
where we let $y=-x$.
\\
\item {[6 points]} If $f\in C[-1,1]$ then
\[
((P_e+P_o)f)(x)=(P_e f)(x) +(P_o f)(x) = {1 \over 2}\left(f(x) + f(-x)\right)+{1 \over 2}\left(f(x) - f(-x)\right) = f(x),
\]
and so
\[
((P_e+P_o)((P_e+P_o)f))(x)= ((P_e+P_o)f)(x).
\]
Hence, $(P_e+P_o)((P_e+P_o)f)=(P_e+P_o)f$ for all $f\in C[-1,1]$ and so $P_e + P_o$ is a projection.
\\
\item {[7 points]} If $f\in C[a,b]$ then
\[
Pf={1\over b-a}B\ip{f,\phi}\phi
\]
and so
\begin{eqnarray*}
P(Pf)&=&{1\over b-a}B\ip{Pf,\phi}\phi.
\end{eqnarray*}
Now,
\begin{eqnarray*}
B\ip{Pf,\phi}&=&\int_a^b{1\over b-a}B\ip{f,\phi}\phi(x)\phi(x)\,dx
\\
&=&\int_a^b{1\over b-a}B\ip{f,\phi}\,dx
\\
&=&B\ip{f,\phi}\int_a^b{1\over b-a}\,dx
\\
&=&B\ip{f,\phi}\left[{x\over b-a}\right]_a^b
\\
&=&B\ip{f,\phi}\left({b\over b-a}-{a\over b-a}\right)
\\
&=&B\ip{f,\phi}{b-a\over b-a}
\\
&=&B\ip{f,\phi}.
\end{eqnarray*}
Consequently,
\begin{eqnarray*}
P(Pf)&=&{1\over b-a}B\ip{Pf,\phi}\phi
\\
&=&{1\over b-a}B\ip{f,\phi}\phi
\\
&=&Pf.
\end{eqnarray*}
Hence, $P(Pf)=Pf$ for all $f\in C[a,b]$ and so $P$ is a projection.
\end{enumerate}
\end{solution}