\begin{solution}
\begin{enumerate}
\item {[13 points]} The properties satisfied by the inner product allow us to say that
\begin{eqnarray*}
a\ip{u-u_N,u-u_N}&=&a\ip{u,u-u_N}-a\ip{u_N,u-u_N}
\\
&=&a\ip{u,u}-a\ip{u,u_N}-a\ip{u_N,u}+a\ip{u_N,u_N}
\\
&=&a\ip{u,u}-2a\ip{u,u_N}+a\ip{u_N,u_N}.
\end{eqnarray*}
Now, $u_N\in V_N$ and so the fact that
\[
a\ip{u_N,v}=\ip{f,v}\mbox{ for all }v\in V_N
\]
means that
\[
a\ip{u_N,u_N}=\ip{f,u_N}.
\]
Moreover, $u_N\in H^1_D(0,1)$, since $V_N$ is a subspace of $H^1_D(0,1)$ and $u_N\in V_N$, and so the fact that
\[
a\ip{u,v}=\ip{f,v}\mbox{ for all }v\in H^1_D(0,1)
\]
means that
\[
a\ip{u,u_N}=\ip{f,u_N}.
\]
So,
\[
a\ip{u,u}-2a\ip{u,u_N}+a\ip{u_N,u_N}=a\ip{u,u}-2\ip{f,u_N}+\ip{f,u_N}=a\ip{u,u}-\ip{f,u_N}.
\]
Therefore,
\[
a\ip{u-u_N,u-u_N}=a\ip{u,u}-\ip{f,u_N}=a\ip{u,u}-a\ip{u_N,u_N}
\]
because
\[
a\ip{u_N,u_N}=\ip{f,u_N}.
\]
\\
\item {[12 points]} We first compute that
\[
\BK\Bc=\Bd
\]
where $\Bd\in\R^{N}$ is the vector with entries
\[
d_j=\sum_{k=1}^Na\ip{\phi_k,\phi_j}c_k
\]
for $j=1,\ldots,N$. Moreover, since
\[
u_N=\sum_{j=1}^Nc_j\phi_j=\sum_{k=1}^Nc_k\phi_k,
\]
the properties satisfied by the inner product yield that
\[
\sum_{k=1}^Na\ip{\phi_k,\phi_j}c_k=a\left(\sum_{k=1}^Nc_k\phi_k,\phi_j\right)=a\ip{u_N,\phi_j}
\]
and so
\[
d_j=a\ip{u_N,\phi_j}
\]
for $j=1,\ldots,N$. Therefore,
\[
\Bc^T\BK\Bc=\Bc^T\Bd=\sum_{j=1}^Nc_ja\ip{u_N,\phi_j}=a\left(u_N,\sum_{j=1}^Nc_j\phi_j\right)=a\ip{u_N,u_N}
\]
by the properties satisfied by the inner product and the fact that
\[
u_N=\sum_{j=1}^Nc_j\phi_j.
\]
\end{enumerate}
\end{solution}