\begin{solution}
\begin{enumerate}
\item {[10 points]} Since,
\[
\lambda\BI-\BA=\left[\begin{array}{cc}\lambda & -1\\1 & \lambda\end{array}\right]
\]
we have that
\[
\det\left(\lambda\BI-\BA\right)=\lambda^2+1
\]
and so
\[
\det\left(\lambda\BI-\BA\right)=0
\]
when $\lambda^2=-1$. Hence, the eigenvalues of $\BA$ are
\[
\lambda_1=-i
\]
and
\[
\lambda_2=i.
\]

Moreover,
\[
\left(\lambda_1\BI-\BA\right)\left[\begin{array}{c}c_1 \\ c_2\end{array}\right]=\left[\begin{array}{cc}-i & -1\\1 & -i\end{array}\right]\left[\begin{array}{c}c_1 \\ c_2\end{array}\right]=\left[\begin{array}{c}-c_1i-c_2 \\ c_1-c_2i\end{array}\right]
\]
and so to make this vector zero we need to set $c_2=-c_1i$. Hence, any vector of the form
\[
\left[\begin{array}{c}c_1 \\ -c_1i\end{array}\right]
\]
where $c_1$ is a nonzero constant is an eigenvector of $\BA$ corresponding to the eigenvalue $\lambda_1$. Let us choose
\[
\Bv_1=\left[\begin{array}{c}1 \\ -i\end{array}\right].
\]

Furthermore,
\[
\left(\lambda_2\BI-\BA\right)\left[\begin{array}{c}d_1 \\ d_2\end{array}\right]=\left[\begin{array}{cc}i & -1\\1 & i\end{array}\right]\left[\begin{array}{c}d_1 \\ d_2\end{array}\right]=\left[\begin{array}{c}d_1i-d_2 \\ d_1+d_2i\end{array}\right]
\]
and so to make this vector zero we need to set $d_2=d_1i$. Hence, any vector of the form
\[
\left[\begin{array}{c}d_1 \\ d_1i\end{array}\right]
\]
where $d_1$ is a nonzero constant is an eigenvector of $\BA$ corresoponding to the eigenvalue $\lambda_2$. Let us choose
\[
\Bv_2=\left[\begin{array}{c}1 \\ i\end{array}\right].
\]

The matrix $\BA$ has eigenvalues $\lambda_1 = -i$ and $\lambda_2 = i$ and eigenvectors
\[
\Bv_1 = \left[\begin{array}{c}1 \\ -i\end{array}\right]
\]
and
\[
\Bv_2 = \left[\begin{array}{c}1 \\ i\end{array}\right]
\]
which are such that $\BA\Bv_1=\lambda_1\Bv_1$ and $\BA\Bv_2=\lambda_2\Bv_2$. If we set
\[
\BV = [\Bv_1\ \Bv_2]=\left[\begin{array}{cc}1 & 1 \\ -i & i\end{array}\right]
\]
and
\[
\BLambda = \left[\begin{array}{cc}\lambda_1 & 0 \\ 0 & \lambda_2\end{array}\right]=\left[\begin{array}{cc}-i & 0 \\ 0 & i\end{array}\right]
\]
then we have that
\[
\BA = \BV\BLambda\BV^{-1}
\]
and
\begin{eqnarray*}
e^{t\BA}&=&\BV e^{t\BLambda} \BV^{-1}
\\
&=&\left[\begin{array}{cc}1 & 1 \\ -i & i\end{array}\right] \left[\begin{array}{cc}e^{-it} & 0 \\ 0 & e^{it}\end{array}\right] \left[\begin{array}{cc}{1\over 2} & {i\over 2} \\ {1\over 2} & -{i\over 2}\end{array}\right]
\\
&=&\left[\begin{array}{cc}e^{-it} & e^{it} \\ -ie^{-it} & ie^{it}\end{array}\right] \left[\begin{array}{cc}{1\over 2} & {i\over 2} \\ {1\over 2} & -{i\over 2}\end{array}\right]
\\
&=&\left[\begin{array}{cc}{1\over2}\left(e^{it} + e^{-it}\right) & {i\over2}\left(e^{-it} - e^{it}\right) \\ {i\over2}\left(e^{it}-e^{-it}\right) & {1\over2}\left(e^{it}+e^{-it}\right)\end{array}\right]
\end{eqnarray*}
since
\[
\BV^{-1}={1 \over i-\left(-i\right)}\left[\begin{array}{cc}i & -1 \\ i & 1\end{array}\right]={1 \over 2i}\left[\begin{array}{cc}i & -1 \\ i & 1\end{array}\right]={-i \over -i}{1 \over 2i}\left[\begin{array}{cc}i & -1 \\ i & 1\end{array}\right]={-i \over 2}\left[\begin{array}{cc}i & -1 \\ i & 1\end{array}\right]=\left[\begin{array}{cc}{1\over 2} & {i\over 2} \\ {1\over 2} & -{i\over 2}\end{array}\right].
\]
Now,
\[
e^{it} + e^{-it}=\cos(t)+i\sin(t)+\cos(t)-i\sin(t)=2\cos(t),
\]
\begin{eqnarray*}
i\left(e^{it} - e^{-it}\right)&=&i\left(\cos(t)+i\sin(t)-\left(\cos(t)-i\sin(t)\right)\right)
\\
&=&i\left(\cos(t)+i\sin(t)-\cos(t)+i\sin(t)\right)
\\
&=&2i^2\sin(t)
\\
&=&-2\sin(t)
\end{eqnarray*}
and
\[
i\left(e^{-it} - e^{it}\right)=-i\left(e^{it} - e^{-it}\right)=2\sin(t).
\]
Therefore,
\[
e^{t\BA} = \left[\begin{array}{cc}\cos(t) & \sin(t) \\ -\sin(t) & \cos(t)\end{array}\right].
\]
Hence,
\[
\Bx(t) = e^{t\BA} \Bx_0 = \left[\begin{array}{cc}\cos(t) & \sin(t) \\ -\sin(t) & \cos(t)\end{array}\right]\left[\begin{array}{c}1 \\ 1\end{array}\right] = \left[\begin{array}{c}\cos(t)+\sin(t) \\ \cos(t)-\sin(t)\end{array}\right].
\]
\\
\item {[5 points]} We can compute that, for each $t\in\R$,
\begin{eqnarray*}
\norm{\Bx(t)}^2&=&\left(\cos(t)+\sin(t)\right)^2+\left(\cos(t)-\sin(t)\right)^2
\\
&=&\left(\cos(t)\right)^2+2\cos(t)\sin(t)+\left(\sin(t)\right)^2+\left(\cos(t)\right)^2-2\cos(t)\sin(t)+\left(\sin(t)\right)^2
\\
&=&2\left(\left(\cos(t)\right)^2+\left(\sin(t)\right)^2\right)
\\
&=&2.
\end{eqnarray*}
Hence, for all  $t\ge0$,
\[
\norm{\Bx(t)}=\sqrt{2}
\]
and so $\norm{\Bx(t)}$ does not change as $t$ increases.
\\
\item {[5 points]} Now,
\[
\Bx_k = (\BI+\Delta t \BA)^k \Bx_0.
\]
Moreover, the eigenvalues of $\BI+\Delta t \BA$ are $1+\Delta t \lambda_1 = 1-\Delta t i$ and $1+\Delta t \lambda_2 = 1+\Delta ti$ and
\[
\BI+\Delta t \BA=\BV \left[\begin{array}{cc}1-\Delta ti & 0 \\ 0 & 1+\Delta ti\end{array}\right] \BV^{-1}.
\]
Furthermore, for all choices of the timestep $\Delta t>0$,
\[
\left|1-\Delta t i\right|=\sqrt{1+\left(\Delta t\right)^2}>1
\]
and
\[
\left|1+\Delta t i\right|=\sqrt{1+\left(\Delta t\right)^2}>1.
\]
Hence, for all choices of the timestep $\Delta t>0$, $\norm{\Bx_k}\rightarrow\infty$ as $k\to\infty$.
\\
\item {[5 points]} Now,
\[
\Bx_k = ((\BI-\Delta t \BA)^{-1})^k \Bx_0.
\]
Moreover, the eigenvalues of $(\BI-\Delta t \BA)^{-1}$ are ${1\over1-\Delta t \lambda_1} = {1\over1+\Delta t i}$ and ${1\over1-\Delta t \lambda_2} = {1\over1-\Delta ti}$ and
\[
(\BI-\Delta t \BA)^{-1}=\BV \left[\begin{array}{cc}{1\over1+\Delta t i} & 0 \\ 0 & {1\over1-\Delta ti}\end{array}\right] \BV^{-1}.
\]
Furthermore, for all choices of the timestep $\Delta t>0$,
\[
\left|{1\over1+\Delta t i}\right|={\left|1\right|\over\left|1+\Delta t i\right|}={1\over\sqrt{1+\left(\Delta t\right)^2}}<1
\]
and
\[
\left|{1\over1-\Delta t i}\right|={\left|1\right|\over\left|1-\Delta t i\right|}={1\over\sqrt{1+\left(\Delta t\right)^2}}<1
\]
since
\[
\sqrt{1+\left(\Delta t\right)^2}>1.
\]
Hence, for all choices of the timestep $\Delta t>0$, $\norm{\Bx_k}\rightarrow0$ as $k\to\infty$.
\end{enumerate}
\end{solution}







