
%In this problem, we will derive a finite difference discretization for slight variations on the steady state heat equation on the interval $[0,1]$.  The motivation for finite difference equations is to satisfy an approximations to the differential equation at a finite number of points $x_i$ by replacing $\pd{u(x_i)}{x}{2}$ with a central finite difference approximation
%\[
%\pd{u(x_i)}{x}{2} \approx \frac{ u_{i+1} - 2u_i + u_{i-1}}{h^2}.
%\]
%where $u_i$ approximates $u(x_i)$ at one the 5 points with spacing $h = 1/4$
%\[
%x_0 = 0, \quad x_1 = \frac{1}{4}, \quad x_2 = \frac{1}{2}, \quad x_3 = \frac{3}{4}, \quad x_4 = 1.
%\]
%\begin{enumerate}
%\item Derive the finite difference equations for 
%\[
%- \pd{u(x)}{x}{2} = f(x), \quad 0<x<1
%\]
%with boundary conditions 
%\[
%%u(0) = u_0, \quad u(1) = u_1,
%u(0) = a, \quad u(1) = b,
%\]
%where $a, b$ are some non-zero (but unspecified) values.  Write down the resulting matrix system for the unknowns $u_1, u_2, u_3$.  Please write your answers in terms of $h$.
%\vspace{1em}
%\item Consider now the case of Neumann boundary conditions on both sides
%\[
%u'(0) = u'(1) = 0.
%\]
%We may approximate these boundary conditions with the forward difference
%\[
%u'(0) = u'(x_0) \approx \frac{u_1-u_0}{h} = 0
%\]
%and the backward difference formula
%\[
%u'(1) = u'(x_{4}) \approx \frac{u_{4}-u_3}{h} = 0.
%\]
%Using these approximations, write down the finite difference equations, and construct explicitly the corresponding matrix system.  Please write your answers in terms of $h$, rather than using the specific values of $x_i$.
%\item Using the specific values of $h$ and $x_i$ given at the beginning of the problem and specific $f(x) = e^x$, set up the matrix equation $Au=b$ for part (b).  Verify that ${\bf e}$ is in the null space of ${A}$, where ${\bf e} = (1,1,1)^T$ is the vector of all ones.  What does this imply about the solution to the system?  
%%\item Consider the case where $\alpha = 0$, or
%%\begin{eqnarray*}
%%-u''(x) &= f(x), \quad 0< x< 1\\
%%u'(0) &= 0\\
%%u'(1) &= 0.
%%\end{eqnarray*}
%\vspace{1em}
%\item Derive the finite difference equations for the following modification of the heat equation:
%\[
%\cos(x) u - \pd{u(x)}{x}{2} = f(x), \quad 0<x<1
%\]
%with boundary conditions 
%\[
%u(0) = u(1) = 0.
%\]
%Write down the finite difference equations and the corresponding matrix system for the unknowns $u_1, u_2, u_3$.  Please write your answers in terms of $h$, rather than using the specific values of $x_i$.


%\end{enumerate}


%%%%%%%%%%%%%%%%%%%%%%%%%%%%%%%%%%%%%%%%%%%%%%%%%%%%%%%%%%%%

%\ifthenelse{\boolean{showsols}}{
%\begin{solution}
\begin{enumerate}
\item The finite difference approximation for second derivative $u''(x)$ around the point $x_i$ can be written by central difference difference scheme
\[
\frac{\partial^2 u}{\partial x^2}(x_i)=u''(x_i)=\frac{u(x_{i+1}) - 2u(x_i) + u(x_{i-1})}{h^2}.
\] 
for $i=1,2,3$.
This leads to three equations:
\begin{eqnarray*}
-\frac{u_{2} - 2u_1 + u_{0}}{h^2} =  f(x_1)\\
-\frac{u_{3} - 2u_2 + u_{1}}{h^2} =  f(x_2)\\
-\frac{u_{4} - 2u_3 + u_{2}}{h^2} =  f(x_3).
\end{eqnarray*}
Since $u(x_0) = u(0) = a$ and $u(x_4) = u(1) = b$, we may substitute those values in to get
\begin{eqnarray*}
\frac{-u_2 + 2u_1}{h^2} &=&  f(x_1) + \frac{a}{h}^2\\
\frac{-u_3 +2u_2 - u_{1}}{h^2} &=&  f(x_2)\\
\frac{2u_3 - u_2}{h^2} &=&  f(x_3) + \frac{b}{h}^2.
\end{eqnarray*}
The resulting matrix system is
\[
\frac{1}{h^2}\left[\begin{array}{ccc}
              2 & -1&0 \\
               -1 & 2 &  -1  \\
                 0 &   -1  & 2 
               \end{array}\right]
               \left[\begin{array}{c}
               u_1\\u_2\\u_3
               \end{array}\right] = 
                              \left[\begin{array}{c}
               f(x_1) + \frac{a}{h^2}\\f(x_2)\\f(x_3) + \frac{b}{h^2}
               \end{array}\right]
\]
\item If we approximate Neumann boundary conditions using finite differences, we have
\[
u_0 = u_1, \qquad u_3 = u_4.
\]
Then, we may substitute these values into the equations:
\begin{eqnarray*}
\frac{-u_{2} + 2u_1 - u_{0}}{h^2} =  f(x_1)\\
\frac{-u_{3} + 2u_2 - u_{1}}{h^2} =  f(x_2)\\
\frac{-u_{4} + 2u_3 - u_{2}}{h^2} =  f(x_3).
\end{eqnarray*}
This reduces to
\begin{eqnarray*}
\frac{-u_{2} + u_1 }{h^2} =  f(x_1)\\
\frac{-u_{3} + 2u_2 - u(x_{1})}{h^2} =  f(x_2)\\
\frac{u_3 - u_{2}}{h^2} =  f(x_3).
\end{eqnarray*}
The corresponding matrix system can be written
\[
\frac{1}{h^2}\left[\begin{array}{ccc}
              1 & -1&0 \\
               -1 & 2 &  -1  \\
                 0 &   -1  & 1 
               \end{array}\right]
               \left[\begin{array}{c}
               u_1\\u_2\\u_3
               \end{array}\right] = 
                              \left[\begin{array}{c}
               f(x_1)\\f(x_2)\\f(x_3) 
               \end{array}\right].
\]
\item Substituting in the specific value of $h = 1/4$ (or $1/h = 4$)
\[
4\left[\begin{array}{ccc}
              1 & -1&0 \\
               -1 & 2 &  -1  \\
                 0 &   -1  & 1 
               \end{array}\right]
               \left[\begin{array}{c}
               u_1\\u_2\\u_3
               \end{array}\right] = 
                              \left[\begin{array}{c}
               e^{x_1}\\e^{x_2}\\e^{x_3}
               \end{array}\right].
\]
If we multiply the system matrix by ${\bf e} = (1,1,1)^T$, we can see that 
\[
4\left[\begin{array}{ccc}
              1 & -1&0 \\
               -1 & 2 &  -1  \\
                 0 &   -1  & 1 
               \end{array}\right]
               \left[\begin{array}{c}
               1\\1\\1
               \end{array}\right]=
                                  \left[\begin{array}{c}
               4(1 - 1)\\ 4(-1 + 2 -1) \\ 4(1-1)
               \end{array}\right] = 
                                  \left[\begin{array}{c}
0\\0\\0
               \end{array}\right].
\]
This implies that the system matrix has a non-trivial nullspace, so that the solution to the finite difference matrix equation is non-unique.
\item The finite difference equations for this modification of the heat equation give
\begin{eqnarray*}
\cos(x_1) u(x_1) + \frac{-u(x_{2}) + 2u(x_1) - u(x_{0})}{h^2} =  f(x_1)\\
\cos(x_2) u(x_2) +\frac{-u(x_{3}) + 2u(x_2) - u(x_{1})}{h^2} =  f(x_2)\\
\cos(x_3) u(x_3) +\frac{-u(x_{4}) + 2u(x_3) - u(x_{2})}{h^2} =  f(x_3).
\end{eqnarray*}
The resulting matrix equation gives
\[
\left(\left[\begin{array}{ccc}
              \cos(x_1) &0 & 0 \\
               0 & \cos(x_2) &  0  \\
                 0 &   0  & \cos(x_3) 
               \end{array}\right] + \frac{1}{h^2}\left[\begin{array}{ccc}
              1 & -1&0 \\
               -1 & 2 &  -1  \\
                 0 &   -1  & 1 
               \end{array}\right]\right)
               \left[\begin{array}{c}
               u_1\\u_2\\u_3
               \end{array}\right] = 
                              \left[\begin{array}{c}
               f(x_1)\\f(x_2)\\f(x_3) 
               \end{array}\right].
\]

\end{enumerate}
%\end{solution}
%}{}
