
Let the symmetric bilinear form $\ip{\cdot,\cdot}:L^2(0,1)\times L^2(0,1)\to\R$ be defined by
\[
\ip{v,w}=\int_0^1v(x)w(x)\,dx
\]
and let the symmetric bilinear form $a\ip{\cdot,\cdot}:H^1(0,1)\times H^1(0,1)\to\R$ be defined by
\[
a\ip{v,w}=\int_0^1v'(x)w'(x)\,dx.
\]
Let $B\ip{\cdot,\cdot}:H^1(0,1)\times H^1(0,1)\to\R$ be defined by
\[
B\ip{v,w}=a\ip{v,w}+\ip{v,w}.
\]
Let the norm $\left|\left|\left|\cdot\right|\right|\right|:H^1(0,1)\to\R$ be defined by
\[
\left|\left|\left|v\right|\right|\right|=\sqrt{B\ip{v,v}}.
\]
Let $f\in L^2(0,1)$, let $\rho\in\R$, let $H^1_D(0,1)=\left\{w\in H^1(0,1):\,w(0)=0\right\}$ and let $u\in H^1_D(0,1)$ be such that
\[
B\ip{u,v}=\ip{f,v}+\rho v(1)\mbox{ for all }v\in H^1_D(0,1).
\]
Moreover, let N be a positive integer, let $V_N$ be a subspace of $H^1_D(0,1)$ and let $u_N\in V_N$ be such that
\[
B\ip{u_N,v}=\ip{f,v}+\rho v(1)\mbox{ for all }v\in V_N.
\]
\\
\begin{enumerate}
\item Use the fact that $\ip{\cdot,\cdot}$ is a symmetric bilinear form on $L^2(0,1)$ and the fact that $a\ip{\cdot,\cdot}$ is a symmetric bilinear form on $H^1(0,1)$ to show that $B\ip{\cdot,\cdot}$ is a symmetric bilinear form on $H^1(0,1)$. Recall that $H^1(0,1)=\left\{v\in L^2(0,1):\,v'\in L^2(0,1)\right\}$.
\\
\item Show that
\[
B\ip{u-u_N,v}=0\mbox{ for all }v\in V_N.
\]
\\
\item Show that
\[
\left|\left|\left|u-u_N\right|\right|\right|^2=\left|\left|\left|u\right|\right|\right|^2-\left|\left|\left|u_N\right|\right|\right|^2.
\]
\\
\item Show that
\[
\left|\left|\left|u_N\right|\right|\right|^2\le\left|\left|\left|u\right|\right|\right|^2.
\]
\end{enumerate}


%%%%%%%%%%%%%%%%%%%%%%%%%%%%%%%%%%%%%%%%%%%%%%%%%%%%%%%%%%%%%%%%%%%%%%%%%%%%%%%%

\ifthenelse{\boolean{showsols}}{\input errfem_sol}{}

