\begin{solution}
\begin{enumerate}
\item $[$8 points] $v(x) = 1/x^2$ is a solution of (1.1).\\      
      To plug $v(x) = 1/x^2$ into the left-hand side of (1.1), we compute
      $dv/dx = d(x^{-2})/dx = -2x^{-3}$.  Substituting this formula,
      the left-hand side of (1.1) becomes 
           \[ -2x^{-3} + 2x^{-1}x^{-2} = 0.\]
      This agrees with the right-hand side of (1.1), so this $v$ is a solution.

\item $[$8 points] $v(x,t) = t(t+x)$ is a solution of (1.2).\\
      We compute $\partial v/\partial t =  2t+x$ and
                 $\partial v/\partial x = t$.
      Thus the left-hand side of (1.2) becomes
        \[ (2t+x) - 3(t) = x-t.\]
      This agrees with the right-hand side of (1.2), so this $v$ is a solution.

\item $[$9 points] $u(x,t) = x e^t$ is \emph{not} a solution of (1.3).\\
       We compute $\partial u /\partial t = xe^t$ and 
       $\partial u/\partial x = e^t$.
       From this it follows that 
           \[ {\partial\over \partial x} \left[ 2u {\partial u\over \partial x}\right]
                = {\partial \over \partial x} 2xe^{2t} = 2e^{2t}.\]
       Thus the left-hand side of (1.3) is
            \[ xe^t -2e^{2t},\]
       which is nonzero in general, in disagreement with the right-hand side of (1.3).
\end{enumerate}


\end{solution}