\begin{solution}
\begin{enumerate}
\item {[20 points]} Since,
\[
\lambda\BI-\BA=\left[\begin{array}{cc}\lambda & -1\\-1 & \lambda\end{array}\right]
\]
we have that
\[
\det\left(\lambda\BI-\BA\right)=\lambda^2-1=\left(\lambda-1\right)\left(\lambda+1\right)
\]
and so
\[
\det\left(\lambda\BI-\BA\right)=0
\]
when $\lambda=-1$ or $\lambda=1$. Hence, the eigenvalues of $\BA$ are
\[
\lambda_1=-1
\]
and
\[
\lambda_2=1.
\]

Moreover,
\[
\left(\lambda_1\BI-\BA\right)\left[\begin{array}{c}c_1 \\ c_2\end{array}\right]=\left[\begin{array}{cc}-1 & -1\\-1 & -1\end{array}\right]\left[\begin{array}{c}c_1 \\ c_2\end{array}\right]=\left[\begin{array}{c}-c_1-c_2 \\ -c_1-c_2\end{array}\right]
\]
and so to make this vector zero we need to set $c_2=-c_1$. Hence, any vector of the form
\[
\left[\begin{array}{c}c_1 \\ -c_1\end{array}\right]
\]
where $c_1$ is a nonzero constant is an eigenvector of $\BA$ corresponding to the eigenvalue $\lambda_1$. Let us choose
\[
\Bv_1=\left[\begin{array}{c}{1\over\sqrt{2}} \\ -{1\over\sqrt{2}}\end{array}\right].
\]

Furthermore,
\[
\left(\lambda_2\BI-\BA\right)\left[\begin{array}{c}d_1 \\ d_2\end{array}\right]=\left[\begin{array}{cc}1 & -1\\-1 & 1\end{array}\right]\left[\begin{array}{c}d_1 \\ d_2\end{array}\right]=\left[\begin{array}{c}d_1-d_2 \\ -d_1+d_2\end{array}\right]
\]
and so to make this vector zero we need to set $d_2=d_1$. Hence, any vector of the form
\[
\left[\begin{array}{c}d_1 \\ d_1\end{array}\right]
\]
where $d_1$ is a nonzero constant is an eigenvector of $\BA$ corresponding to the eigenvalue $\lambda_2$. Let us choose
\[
\Bv_2=\left[\begin{array}{c}{1\over\sqrt{2}} \\ {1\over\sqrt{2}}\end{array}\right].
\]

The matrix $\BA$ has eigenvalues $\lambda_1 = -1$ and $\lambda_2 = 1$ and eigenvectors
\[
\Bv_1 = \left[\begin{array}{c}{1\over\sqrt{2}} \\ -{1\over\sqrt{2}}\end{array}\right]
\]
and
\[
\Bv_2 = \left[\begin{array}{c}{1\over\sqrt{2}} \\ {1\over\sqrt{2}}\end{array}\right]
\]
which are such that $\BA\Bv_1=\lambda_1\Bv_1$, $\BA\Bv_2=\lambda_2\Bv_2$, $\Bv_1\cdot\Bv_1=\Bv_2\cdot\Bv_2=1$,  and $\Bv_1\cdot\Bv_2=\Bv_2\cdot\Bv_1=0$. Since $\BA=\BA^T$, if we set
\[
\BV = [\Bv_1\ \Bv_2]=\left[\begin{array}{cc}{1\over\sqrt{2}} & {1\over\sqrt{2}} \\ -{1\over\sqrt{2}} & {1\over\sqrt{2}}\end{array}\right]
\]
and
\[
\BLambda = \left[\begin{array}{cc}\lambda_1 & 0 \\ 0 & \lambda_2\end{array}\right]=\left[\begin{array}{cc}-1 & 0 \\ 0 & 1\end{array}\right]
\]
then we have that
\[
\BA = \BV\BLambda\BV^T
\]
and
\begin{eqnarray*}
e^{t\BA} &=& \BV e^{t\BLambda} \BV^T
\\
&=& \left[\begin{array}{cc}{1\over\sqrt{2}} & {1\over\sqrt{2}} \\ -{1\over\sqrt{2}} & {1\over\sqrt{2}}\end{array}\right] \left[\begin{array}{cc}e^{-t} & 0 \\ 0 & e^{t}\end{array}\right] \left[\begin{array}{cc}{1\over\sqrt{2}} & -{1\over\sqrt{2}} \\ {1\over\sqrt{2}} & {1\over\sqrt{2}}\end{array}\right]
\\
&=& \left[\begin{array}{cc}{1\over\sqrt{2}}e^{-t} & {1\over\sqrt{2}}e^t \\ -{1\over\sqrt{2}}e^{-t} & {1\over\sqrt{2}}e^t\end{array}\right] \left[\begin{array}{cc}{1\over\sqrt{2}} & -{1\over\sqrt{2}} \\ {1\over\sqrt{2}} & {1\over\sqrt{2}}\end{array}\right]
\\
&=& \left[\begin{array}{cc}{1\over2}\left(e^t+e^{-t}\right) & {1\over2}\left(e^t - e^{-t}\right) \\ {1\over2}\left(e^t-e^{-t}\right) & {1\over2}\left(e^{t}+e^{-t}\right)\end{array}\right].
\end{eqnarray*}
Hence,
\[
\Bx(t) = e^{t\BA} \Bx_0 = \left[\begin{array}{cc}{1\over2}\left(e^t+e^{-t}\right) & {1\over2}\left(e^t - e^{-t}\right) \\ {1\over2}\left(e^t-e^{-t}\right) & {1\over2}\left(e^{t}+e^{-t}\right)\end{array}\right]\left[\begin{array}{c}2 \\ 0\end{array}\right] = \left[\begin{array}{c}e^t+e^{-t} \\ e^t-e^{-t}\end{array}\right].
\]
\\
\item {[5 points]} Since $\lambda_2>0$ and $\Bv_2\cdot\Bx_0={2\over\sqrt{2}}\ne0$, $\norm{\Bx(t)}\rightarrow\infty$ as $t\rightarrow\infty$.
\end{enumerate}
\end{solution}