\begin{solution}
\begin{enumerate}
\item {[7 points]} We first compute that
\[
\BM\Bw=\Bg
\]
where $\Bg\in\R^{N}$ is the vector with entries
\[
g_j=\sum_{k=1}^N\ip{\phi_k,\phi_j}w_k
\]
for $j=1,\ldots,N$. Moreover, since
\[
\hat{w}_N=\sum_{j=1}^Nw_j\phi_j=\sum_{k=1}^Nw_k\phi_k,
\]
the properties satisfied by the inner product yield that
\[
\sum_{k=1}^N\ip{\phi_k,\phi_j}w_k=\left(\sum_{k=1}^Nw_k\phi_k,\phi_j\right)=\ip{\hat{w}_N,\phi_j}
\]
and so
\[
g_j=\ip{\hat{w}_N,\phi_j}
\]
for $j=1,\ldots,N$. Therefore,
\[
\Bw^T\BM\Bw=\Bw^T\Bg=\sum_{j=1}^Nw_j\ip{\hat{w}_N,\phi_j}=\left(\hat{w}_N,\sum_{j=1}^Nw_j\phi_j\right)=\ip{\hat{w}_N,\hat{w}_N}
\]
by the properties satisfied by the inner product and the fact that
\[
\hat{w}_N=\sum_{j=1}^Nw_j\phi_j.
\]
\\
\item {[8 points]} If $\BM^{-1}\BK\Bw=\lambda\Bw$, for $\lambda\in\R$ and $\Bw\in\R^N$, then
\[
\BK\Bw=\lambda\BM\Bw
\]
and hence
\[
\Bw^T\BK\Bw=\lambda\Bw^T\BM\Bw
\]
from which it follows that
\[
a\ip{\hat{w}_N,\hat{w}_N}=\lambda\ip{\hat{w}_N,\hat{w}_N}
\]
using the information given in parts (a) and (b).
\\
\item {[10 points]} Let $\lambda\in\R$ be an eigenvalue of $\BM^{-1}\BK$. Then there exist nonzero $\Bv\in\R^N$ which are such that
\[
\BM^{-1}\BK\Bv=\lambda\Bv.
\]
Let $\Bw\in\R^N$ be such that
\[
\BM^{-1}\BK\Bw=\lambda\Bw
\]
and $\Bw\ne\Bzero$. From part (b) we then have that
\[
a\ip{\hat{w}_N,\hat{w}_N}=\lambda\ip{\hat{w}_N,\hat{w}_N}.
\]
Moreover, since $\Bw\ne\Bzero$ then $\hat{w}_N\ne 0$ because $\{\phi_1,...,\phi_N\}$ is linearly independent. Hence, since $\hat{w}_N\ne 0$, the properties satisfied by an inner product mean that $a\ip{\hat{w}_N,\hat{w}_N}>0$ and so
\[
\lambda\ip{\hat{w}_N,\hat{w}_N}>0.
\]
Consequently, 
\[
\lambda>0
\]
since, because $\hat{w}_N\ne 0$, the properties satisfied by an inner product mean that $\ip{\hat{w}_N,\hat{w}_N}>0$.
\end{enumerate}
\end{solution}