\begin{solution}
\begin{enumerate}
\item {[5 points]} Suppose $\Bu, \Bv \in \Rn$.  Then 
\[
f(\Bu+\Bv) = \BA(\Bu+\Bv) + \Bb  = \BA\Bu + \BA\Bv + \Bb
\]
but
\[
f(\Bu)+f(\Bv) = \BA\Bu + \Bb + \BA\Bv + \Bb = \BA\Bu + \BA\Bv + 2\Bb
\]
and so $f(\Bu+\Bv)$ does not equal $f(\Bu) + f(\Bv)$ when $\Bb\ne \Bzero$. Hence, $f$ \emph{is not} a linear operator.
\\
\item {[5 points]} Suppose $\Bx\in \Rn$ and $\alpha\in\R$. Then 
\[
f(\alpha\Bx) = (\alpha \Bx)^T(\alpha \Bx) = \alpha^2 \Bx^T\Bx
\]
and 
\[
\alpha f(\Bx) = \alpha \Bx^T\Bx.
\]
However, if $\displaystyle{\Bx = \left[\begin{array}{c}1\\ 0\end{array}\right]}$ and $\alpha=2$ then $\Bx^T\Bx=1$ and so
\[
f(\alpha\Bx) = 2^2=4
\]
but
\[
\alpha f(\Bx) = 2.
\]
Hence, $f$ \emph{is not} a linear operator.
\\
\item {[5 points]} Suppose $\BX, \BY \in \Rnn$. Then 
\[
f(\BX+\BY) = \BA(\BX+\BY) + (\BX+\BY)\BB = \BA\BX + \BX \BB + \BA\BY + \BY\BB = f(\BX) + f(\BY),
\]
and if $\alpha\in\R$, then
\[
f(\alpha \BX) = \BA(\alpha\BX) + (\alpha \BX) \BB = \alpha (\BA\BX + \BX\BB) = \alpha f(\BX).
\]
Hence, $f$ \emph{is} a linear operator.
\\
\item {[5 points]} Suppose that $u \in C^1[0,1]$ and $\alpha \in \R$. Then 
\[
\alpha(Lu)(x) = \alpha u(x) u'(x)
\]
and
\[
(L(\alpha u))(x) = (\alpha u)(x) (\alpha u)'(x)=\alpha^2u(x) u'(x).
\]
However, if $u(x) = x$ and $\alpha=2$ then
\[
\alpha(Lu)(x) = 2x
\]
but
\[
(L(\alpha u))(x) = 2^2 x=4x.
\]
Hence, $L$ \emph{is not} a linear operator.
\\
\item {[5 points]} Suppose that $u, v \in C^2[0,1]$. Then 
\begin{eqnarray*}
(L(u+v))(x) &=& (u+v)''(x) - \sin(x) (u+v)'(x) + \cos(x) (u+v)(x)
\\
&=& u''(x) - \sin(x) u'(x) + \cos(x) u(x) + v''(x) - \sin(x) v'(x) + \cos(x) v(x)
\\
&=& (Lu)(x) + (Lv)(x),
\end{eqnarray*}
and for all $\alpha \in \R$,
\begin{eqnarray*}
(L(\alpha u))(x) &=& (\alpha u)''(x) - \sin(x) (\alpha u)'(x) + \cos(x) (\alpha u)(x)
\\
&=& \alpha \left(u''(x) - \sin(x) u'(x) + \cos(x) u(x)\right)
\\
&=& \alpha (Lu)(x).
\end{eqnarray*}
Hence, $L$ \emph{is} a linear operator.
\end{enumerate}
\end{solution}